prove modulus of product of modulus is preserved

math/division.dfy
@@ -39,6 +39,15 @@ lemma selfAnnihilation(a: int, b: int)
 //    assert x * a == b;
 // }
 
+lemma DivisionTheoremNat(a: nat, b: nat)
+    requires a != 0
+    requires b % a == 0
+    ensures exists x :: x * a == b
+{
+   var x := b / a;
+   assert x * a == b;
+}
+
 lemma DivisionTheorem(a: int, b: int)
     requires a != 0
     requires b % a == 0
@@ -59,15 +68,42 @@ lemma divCancel(x: int, a: int)
 //     }
 // }
 
-lemma remainderSubtract(x: int, a: int, c: int) 
+lemma remainderSubtract(x: int, a: int, c: nat) 
     requires a != 0
     requires c == x % a
     ensures (x-c) % a == 0
+{
+    // if(a > x) {
+    //     assert x % a == x;
+    //     assert c == x;
+    //     var z := 0;
+    //     assert z * a + c == x;
+    // }else if(a == x) {
+    //     assert x % a == 0;
+    //     var z := 0;
+    //     assert c == 0;
+    //     assert z*a + c == 0;
+    // } else {
+    //     assert a < x;
+    //     var k := x / a;
+    //     assert k >= 1;
+    //     assert x == k * a + c;
+    // }
+    var q := x / a;
+    assert x - c == q * a;
+    selfAnnihilation(a, q);
+    // assert x == x/a + c;
+}
 // {
 // }
 
+function {:opaque} prod(x: int, y: int): int {
+    x * y
+}
+
 function divAdd(b: int, a: int, c: int): int {
-    b * a + c
+    // reveal prod();
+    prod(b,a) + c
 }
 
 lemma remainderTheorem(x: int, a: int, c: int)
@@ -77,6 +113,7 @@ lemma remainderTheorem(x: int, a: int, c: int)
 {
    var q := (x-c) / a;
    remainderSubtract(x,a,c);
+   reveal prod();
 //    calc {
 //        q * a + c;
 //        ((x-c)/a) * a + c;
@@ -86,6 +123,18 @@ lemma remainderTheorem(x: int, a: int, c: int)
 //    }
    assert divAdd(q,a,c) == x;
 }
+
+lemma remainderTheorem2(x: int, a: int)
+    requires a != 0
+    ensures exists q,c :: divAdd(q,a,c) == x && c == x % a;
+{
+   var c := x % a;
+   var q := (x-c) / a;
+   remainderSubtract(x,a,c);
+   reveal prod();
+   assert divAdd(q,a,c) == x;
+}
+
 
 lemma dpOne(a: int, b: int, c: int) 
     requires a != 0
@@ -120,6 +169,7 @@ lemma xsquaredminusOne(x: int)
     if x % 3 == 1 {
         remainderTheorem(x, 3, 1);
         var q: int :| divAdd(q,3,1) == x;
+        reveal prod();
         calc {
             x*x-1;
             (3*q+1)*(3*q+1)-1;
@@ -133,6 +183,7 @@ lemma xsquaredminusOne(x: int)
     if x % 3 == 2 {
         remainderTheorem(x, 3, 2);
         var p :| divAdd(p,3,2) == x;
+        reveal prod();
         calc {
             x*x-1;
             (3*p+2)*(3*p+2)-1;
@@ -199,6 +250,7 @@ lemma smuh(A: iset<int>, B: iset<int>)
         assert n % 4 == 3;
         remainderTheorem(n,4,3);
         var q :| divAdd(q,4,3) == n;
+        reveal prod();
         assert n == 2*(2*q+1)+1;
         // selfAnnihilation(2,2*q+1);
         assert 2*(2*q+1) % 2 == 0;
@@ -211,3 +263,87 @@ lemma smuh(A: iset<int>, B: iset<int>)
 lemma modPlus(a: int, b: int, n: int)
     requires n != 0;
     ensures ((a % n) + (b % n)) % n == (a + b) % n
+
+/*
+https://math.stackexchange.com/questions/882953/a-equiv-bar-a-pmod-kn-rightarrow-a-equiv-bar-a-pmod-n-a-bmod-k
+Suppose 𝑎≡𝑏mod𝑝𝑞 and 𝑏≡𝑐mod𝑝, then we have
+𝑎=𝑟𝑝𝑞+𝑏=𝑟𝑝𝑞+(𝑠𝑝+𝑐)=(𝑟𝑞+𝑠)𝑝+𝑐
+so that 𝑎≡𝑐mod𝑝
+*/
+
+lemma prodCommutes(a: int, b: int)
+    ensures prod(a,b) == prod(b,a)
+{
+    reveal prod();
+}
+
+lemma prodCommutesThree(a: int, b: int, c: int) 
+    ensures prod(a, prod(b, c)) == prod(b, prod(a, c))
+{
+    reveal prod();
+}
+
+lemma prodDistributes(a: int, b: int, c: int)
+    ensures prod(a, b + c) == prod(a,b) + prod(a,c)
+{
+    reveal prod();
+}
+
+lemma prodSelfAnnihilation(a: int, b: int) 
+    requires a != 0
+    ensures prod(a,b) % a == 0
+{
+    reveal prod();
+    calc {
+        (b * a) % a;
+        {modMultiplication(a,0,b,b%a,a);}
+        (0 * b%a) % a;
+        0;
+    }
+}
+
+lemma congruencePersistMod(a: nat, b: nat, p: nat, q: nat, c: nat)
+    requires p != 0
+    requires q != 0
+    requires prod(p,q) != 0
+    requires a % prod(p,q) == b;
+    requires b % p == c;
+
+    ensures a % p == c
+{
+    assert c % p == c;
+    remainderTheorem(a, prod(p,q), b);
+    var r :| divAdd(r, prod(p,q), b) == a;
+    remainderTheorem(b, p, c);
+    var s :| divAdd(s, p, c) == b;
+    calc {
+        a % p;
+        (prod(r, prod(p,q)) + b) % p;
+        (prod(r, prod(p,q)) + prod(s, p) + c) % p;
+        == {prodCommutes(s,p);}
+        (prod(r, prod(p,q)) + prod(p, s) + c) % p;
+        == {prodCommutesThree(r, p, q);}
+        (prod(p, prod(r,q)) + prod(p, s) + c) % p;
+        == {prodDistributes(p,prod(r,q),s);}
+        (prod(p, prod(r,q) + s) + c) % p;
+        == {modPlus(prod(p, prod(r,q) + s),c,p);}
+        (prod(p, prod(r,q) + s) % p + c % p) % p;
+        (prod(p, prod(r,q) + s) % p + c) % p;
+        == {prodSelfAnnihilation(p, prod(r,q) + s);}
+        (0 + c) % p;
+        c % p; 
+        c;
+    }
+}
+    // calc {
+    //     a % p;
+    //     (r * p * q + b) % p;
+    //     (r * p * q + s*p + c) % p;
+    //     (p*(r*q+s) + c) % p;
+    //     == {modPlus(p*(r*q+s), c, p);}
+    //     ( ((p*(r*q+ s)) % p) + (c % p)) % p;
+    //     == {selfAnnihilation(p, (r*q+s));}
+    //     (0 + c % p) % p;
+    //     c % p;
+    //     c;
+    // }
