math/Artin2_1.dfy
@@ -1,0 +1,60 @@
+
+//!A signifies type invariance
+datatype Group<!A> = Group(elements: set<A>, identity: A, compose: (A,A) -> A)
+
+predicate isIdentity<A>(g: Group<A>) {
+    forall a :: a in g.elements ==> g.compose(a,g.identity) == a && g.compose(g.identity, a) == a
+}
+
+predicate closedComposition<A>(g: Group<A>) {
+    forall x,y :: x in g.elements && y in g.elements ==> g.compose(x,y) in g.elements
+}
+
+predicate associativeComposition<A>(g: Group<A>) {
+    forall a,b,c :: a in g.elements && b in g.elements && c in g.elements ==> g.compose(g.compose(a,b),c) == g.compose(a, g.compose(b,c))
+}
+
+predicate commutativeComposition<A>(g: Group<A>) {
+    forall a,b :: a in g.elements && b in g.elements ==> g.compose(a,b) == g.compose(b,a)
+}
+
+predicate containsInverses<A>(g: Group<A>) {
+    forall x :: x in g.elements ==> exists xbar :: xbar in g.elements && g.compose(x,xbar) == g.identity
+}
+
+predicate ValidGroup<A>(g: Group<A>) {
+    g.identity in g.elements &&
+    isIdentity(g) &&
+    closedComposition(g) &&
+    associativeComposition(g) && 
+    containsInverses(g)
+}
+
+predicate AbelianGroup<A>(g: Group<A>) {
+    ValidGroup(g) && commutativeComposition(g)
+}
+
+lemma groupCompositionInverse<A>(g: Group<A>, a: A, b: A, abar: A, bbar: A, abbar: A) 
+    requires ValidGroup(g)
+    requires a in g.elements
+    requires b in g.elements
+    requires abar in g.elements
+    requires bbar in g.elements
+    requires abbar in g.elements
+    requires g.compose(a, abar) == g.identity
+    requires g.compose(b, bbar) == g.identity
+    requires g.compose(g.compose(a, b), abbar) == g.identity
+    ensures abbar == g.compose(bbar, abar)
+{
+    calc {
+        g.compose(g.compose(a, b), g.compose(bbar, abar));
+        == 
+        g.compose(a, g.compose(g.compose(b, bbar),abar));
+        ==
+        g.compose(a, g.compose(g.identity,abar));
+        ==
+        g.compose(a, abar);
+        ==
+        g.identity;
+    }
+}
