math/betterInjective.dfy
@@ -1,0 +1,135 @@
+// https://stackoverflow.com/questions/74632153/defining-a-surjective-predicate-for-maps-and-functions/74661338#74661338
+// Note: to be useful, the function's type should be --> (a broken arrow)
+// indicating the function CAN have preconditions.
+// Otherwise, -> is already a subset type of --> whose constraint is exactly your predicate
+// so it would be a typing issue to provide a non-total function.
+// See https://dafny.org/latest/DafnyRef/DafnyRef#sec-arrow-subset-types
+predicate isTotal<G(!new), B(!new)>(f:G --> B)
+//    reads f.reads   // You don't need this, because f is not declared as being able to read a function
+{
+    forall g:G :: f.requires(g)
+}
+
+// Passthrough identity function used for triggers
+function Id<T>(t: T): T { t }
+
+predicate Surjective<A(!new), B(!new)>(f: A -> B) 
+{
+    // If not using Id(b), the first forall does not have a trigger
+    // and get hard to prove. Not impossible, but extremely lengthy
+    forall b: B :: exists a: A :: f(a) == Id(b)
+}
+
+predicate isTotalMap<G(!new), B(!new)>(m:map<G,B>)
+{
+     forall g: G :: g in m
+}
+
+predicate mapSurjective<U(!new), V(!new)>(m: map<U,V>)
+    requires forall u: U :: u in m.Keys
+{
+    // If not using Id(b), the first forall does not have a trigger
+    // and get hard to prove. Not impossible, but extremely lengthy
+    forall x: V :: exists a: U :: m[a] == Id(x)
+}
+
+datatype Color = Blue | Yellow | Green | Red
+
+function toRed(x: Color): Color {
+    Red
+}
+
+function shiftColor(x: Color): Color {
+    match x {
+        case Red => Blue
+        case Blue => Yellow
+        case Yellow => Green
+        case Green => Red
+    }
+}
+function partialFunction(x: Color): Color
+  requires x.Red? {
+  x
+}
+
+lemma TestWrong() {
+  // When trying to prove an assertion with a proof, use assert ... by like this:
+  assert !isTotal(partialFunction) by {
+    // If we were using ->, we would get "Value does not satisfies Color -> Color"*
+    // But here we can just exhibit a counter-example that disproves the forall 
+    assert !partialFunction.requires(Blue);
+
+    // A longer proof could be done by contradiction like this:
+    if(isTotal(partialFunction)) {
+      assert forall c: Color :: partialFunction.requires(c);
+      assert partialFunction.requires(Blue); // it can instantiate the forall above.
+      assert false; // We get a contradiction
+    }
+    assert !isTotal(partialFunction);// A ==> false means !A
+  }
+}
+
+lemma TestSurjective() {
+    assert isTotal(toRed);
+    assert isTotal(shiftColor);
+    var toRedm := map[Red := Red, Blue := Red, Yellow := Red, Green := Red];
+    var toShiftm := map[Red := Blue, Blue := Yellow, Yellow := Green, Green := Red];
+    assert !Surjective(toRed) by {
+      if(Surjective(toRed)) {
+        var _ := Id(Blue);
+      }
+    }
+    assert Surjective(shiftColor) by {
+      if(!Surjective(shiftColor)) {
+        var _ := Id(Blue); // We need to trigger the condition of surjective so that Dafny is happy with the below:
+        assert !forall b: Color :: exists a: Color :: shiftColor(a) == Id(b);
+        assert exists b: Color :: forall a: Color :: shiftColor(a) != Id(b);
+        var b : Color :| forall a: Color :: shiftColor(a) != Id(b);
+        assert shiftColor(shiftColor(shiftColor(shiftColor(b)))) == Id(b);
+        assert false;
+      }
+    }
+    assert forall c: Color :: c in toRedm by {
+      if(!forall c :: c in toRedm) {
+        assert exists c :: c !in toRedm;
+        var c :| c !in toRedm;
+        assert c != Red;// Dafny picks up from here
+        assert false;
+      }
+    }
+    assert !mapSurjective(toRedm) by {
+      if(mapSurjective(toRedm)) {
+        assert forall x :: exists a :: toRedm[a] == Id(x);
+        var _ := Id(Blue); // Will instantiate the axiom above with x == Blue
+        assert exists a :: toRedm[a] == Id(Blue); // Not needed, but Dafny can prove this.
+        assert false;
+      }
+    }
+    assert forall u: Color :: u in toShiftm.Keys by {
+      if(!forall u: Color :: u in toShiftm.Keys) {
+        assert exists u :: u !in toShiftm.Keys;
+        var u :| u !in toShiftm.Keys;
+        assert u != Red; // Dafny can pick up from here
+        assert false;
+      }
+    }
+    assert isTotalMap(toShiftm); //also fails
+    assert forall u: Color :: u in toShiftm.Keys;
+    assert mapSurjective(toShiftm) by {
+      if(!mapSurjective(toShiftm)) {
+        var _ := Id(Red); // Necessary so that Dafny understands that the next forall is equivalent
+        assert !forall x :: exists a :: toShiftm[a] == Id(x);
+        assert exists x :: forall a :: toShiftm[a] != Id(x);
+        var x :| forall a :: toShiftm[a] != Id(x);
+        assert forall b :: exists a :: toShiftm[a] == Id(b) by {
+          forall b: Color ensures exists a :: toShiftm[a] == Id(b) {
+            var a := toShiftm[toShiftm[toShiftm[b]]];
+            assert toShiftm[toShiftm[toShiftm[toShiftm[b]]]] == Id(b);
+          }
+        }
+        assert exists a :: toShiftm[a] == Id(x);
+        var b :| toShiftm[b] == Id(x);
+        assert false;
+      }
+    }
+}
