math/pinter_six.dfy
@@ -1,0 +1,250 @@
+
+predicate Injective<A(!new), B>(f: A -> B)
+{
+    forall x, y :: x != y ==> f(x) != f(y)
+}
+predicate isTotal<G(!new), B(!new)>(f:G -> B)
+    reads f.reads;
+{
+     forall g:G :: f.requires(g)
+}
+
+predicate Surjective<A(!new), B(!new)>(f: A -> B) 
+    reads f.reads;
+    // requires isTotal(f)
+{
+    forall b: B :: exists a: A :: f(a) == b 
+}
+
+predicate Bijective<A(!new), B(!new)>(f: A -> B) 
+{
+    Injective(f) && Surjective(f)
+}
+// predicate surjectivee<G>(f : G -> set<G> )  {
+//      forall v : set<G>  :: (exists g:G :: f(g) == v && isSubset(v) )
+// }
+//reads f.reads; requires forall t:: f.requires(t) // f is a total function
+//ensures forall v : set :: (exists u:G :: f(u) == v)
+// map m is injective if no two keys map to the same value	
+predicate mapInjective<U,V>(m: map<U,V>)
+{
+	forall a,b :: a in m && b in m ==> a != b ==> m[a] != m[b]
+}
+
+predicate isTotalMap<G(!new), B(!new)>(m:map<G,B>)
+{
+     forall g:G :: g in m
+}
+
+predicate mapHasValue<U(!new), V(!new)>(m: map<U,V>, x: V)
+{
+    exists a: U :: a in m && m[a] == x
+}
+
+predicate mapSurjective<U(!new), V(!new)>(m: map<U,V>)
+    // requires forall u: U :: u in m.Keys
+    requires isTotalMap(m)
+{
+    forall x: V :: x in m.Values
+    // forall x: V :: mapHasValue(m, x)
+}
+
+// the domain of a map is the set of its keys  
+function domain<U,V>(m: map<U,V>) : set<U>
+	ensures domain(m) == set u : U | u in m :: u;
+	ensures forall u :: u in domain(m) ==> u in m;
+    ensures domain(m) == m.Keys
+{
+		set u : U | u in m :: u
+}
+ 
+// the domain of a map is the set of its values
+function range<U,V>(m: map<U,V>) : set<V>
+	ensures range(m) == set u : U | u in m :: m[u];
+	ensures forall v :: v in range(m) ==> exists u :: u in m && m[u] == v;
+    ensures forall k :: k in m ==> m[k] in range(m)
+    ensures range(m) == m.Values
+{
+	set u : U | u in m :: m[u]
+}
+
+function frange<U(!new),V(!new)>(f: U -> V): iset<V>
+{
+    iset u: U | true :: f(u) 
+}
+
+lemma InjectiveCompositionImpliesInjective<A(!new), B(!new), C(!new)>(f: A -> B, g: B -> C,  h: A -> C)
+    requires h == (x => g(f(x)))
+    requires Injective(h)
+    ensures Injective(f)
+{
+    if !Injective(f) {
+        var x: A, y: A :| x != y && f(x) == f(y);
+        assert h(x) == h(y);
+        assert false;
+    }
+}
+
+lemma SurjectiveCompositionImpliesSurjective<A(!new), B(!new), C(!new)>(f: A -> B, g: B -> C,  h: A -> C)
+    // requires isTotal(f) && isTotal(g) && isTotal(h)
+    requires h == (x => g(f(x)))
+    requires Surjective(h)
+    ensures Surjective(g)
+{
+    // var x: A :| assume true;
+    // var y: A :| assume y != x;
+}
+
+lemma InjectiveAlsoSurjective<A>(f: A -> A)
+    requires Injective(f)
+    ensures Surjective(f)
+{
+    // if !Injective(f) {
+    //     var x: A, y: A :| x != y && f(x) == f(y);
+    //     assert false;
+    // }
+    // forall a: A | true 
+    //     ensures exists b:A :: f(b) == a
+    // {
+    //     if(f(a) == a) {
+
+    //     }else{
+    //         var b := f(a);
+    //     }
+    // }
+    // if !Surjective(f) {
+    //     var missing: A :| forall a: A :: f(a) != missing; 
+    //     assert f(missing) != missing;
+    //     var someresult := f(missing);
+    //     var somex: A :| f(somex) == someresult && somex != missing;
+    // }
+}
+
+lemma bijectiveComposition<A(!new), B(!new), C(!new)>(f: A -> B, g: B -> C,  h: A -> C)
+    requires h == (x => g(f(x)))
+    requires Injective(f)
+    requires Surjective(g)
+    ensures Bijective(h)
+{
+    assert Surjective(h);
+}
+
+datatype Color = Blue | Yellow | Green | Red
+
+function toRed(x: Color): Color {
+    Red
+}
+
+function shiftColor(x: Color): Color {
+    match x {
+        case Red => Blue
+        case Blue => Yellow
+        case Yellow => Green
+        case Green => Red
+    }
+}
+
+method TestSurjectiveMap() {
+    var hmm := map[Red := Red];
+    // TotalColorMapIsTotal(hmm);
+    var toRedm := map[Red := Red, Blue := Red, Yellow := Red, Green := Red];
+    assert toRedm.Keys == {Red, Blue, Yellow, Green};
+    assert toRedm.Values == {Red};
+    // assert forall u: Color :: u in toRedm;
+    TotalColorMapIsTotal(toRedm);
+    assert isTotalMap(toRedm);
+
+    // assert mapSurjective(toRedm);
+    // assert toShiftm.Values == {Blue, Yellow, Green, Red};
+    var toShiftm := map[Red := Blue, Blue := Yellow, Yellow := Green, Green := Red];
+    assert toShiftm[Red] == Blue;
+    assert toShiftm[Blue] == Yellow;
+    assert toShiftm[Yellow] == Green;
+    assert toShiftm[Green] == Red;
+
+    TotalColorMapIsTotal(toShiftm);
+    ColorMapIsOnto(toShiftm);
+    assert mapSurjective(toShiftm);
+}
+
+method testSurjective() {
+    assert isTotal(toRed);
+    assert isTotal(shiftColor);
+
+    assert toRed(Green) == Red;
+    assert toRed(Red) == Red;
+    assert toRed(Blue) == Red;
+    assert toRed(Yellow) == Red;
+    // assert Surjective(toRed); //should fail
+    var test := iset{Red, Blue, Green, Yellow};
+    // assert Red in test;
+    // var quoi := frange(shiftColor);
+    // assert test == frange(shiftColor);
+    // assert exists u: Color :: shiftColor(u) == Red;
+
+    assert shiftColor(Green) == Red;
+    assert shiftColor(Red) == Blue;
+    assert shiftColor(Blue) == Yellow;
+    assert shiftColor(Yellow) == Green;
+    assert Surjective(shiftColor); //should succeed
+}
+
+
+
+
+function toShiftm(): map<Color, Color>
+    ensures Red in toShiftm();
+    ensures Blue in toShiftm();
+    ensures Yellow in toShiftm();
+    ensures Green in toShiftm();
+
+    ensures Red in range(toShiftm());
+    ensures Blue in range(toShiftm());
+    ensures Yellow in range(toShiftm());
+    ensures Green in range(toShiftm());
+    ensures toShiftm().Keys == {Red, Blue, Yellow, Green}
+    ensures toShiftm().Values == {Red, Blue, Yellow, Green}
+    ensures |toShiftm()| == 4
+    // ensures isTotalMap(toShiftm())
+    // ensures forall x : Color :: x in  (set u : Color :: u) ==> x in toShiftm()
+{
+
+    var dom := map[Red := Blue, Blue := Yellow, Yellow := Green, Green := Red];
+    assert |dom.Keys| == 4;
+    // assert forall x: Color :: x in {Blue, Red, Yellow, Green} && x in dom;
+    dom
+}
+
+lemma mapKeysAreEquivalent<A, B>(m: map<A,B>)
+    ensures |m| == |m.Keys|
+{
+
+}
+
+lemma TotalColorMapIsTotal<B>(m: map<Color, B>) 
+    requires m.Keys == {Red, Blue, Green, Yellow}
+    // ensures forall u: Color :: u in m
+    ensures isTotalMap(m)
+{
+    forall u: Color | true
+        ensures u in m
+    {
+        if u.Red? {
+            assert u in m;
+        }
+    }
+}
+
+lemma ColorMapIsOnto<A>(m: map<A, Color>) 
+    requires m.Values == {Red, Blue, Green, Yellow}
+    ensures forall u: Color :: u in m.Values
+{
+
+    forall u: Color | true
+        ensures u in m.Values
+    {
+        if u.Red? {
+            assert u in m.Values;
+        }
+    }
+}
